Ajout record

src/Step.v
@@ -10,128 +10,155 @@ Require Maps.
 Import Maps.Notations.
 
 Inductive step : expr -> expr -> Prop := 
-    | ST_App_Fun : 
-        ∀ (x : string) (t : type) (e e' v : expr),
-        value v -> 
-        substitution v x e e' ->
-        step (E_App (E_Fun x t e) v) e'
-    | ST_App_Left : 
-        ∀ (e1 e1' e2 : expr),
-        step e1 e1' ->
-        step (E_App e1 e2) (E_App e1' e2)
-    | ST_App_Right : 
-        ∀ (v1 e2 e2' : expr),
-        value v1 ->
-        step e2 e2' ->
-        step (E_App v1 e2) (E_App v1 e2')
-    | ST_If_True : 
-        ∀ (e1 e2 : expr),
-        step (E_If E_True e1 e2) e1
-    | ST_If_False : 
-        ∀ (e1 e2 : expr),
-        step (E_If E_False e1 e2) e2
-    | ST_If : 
-        ∀ (e1 e1' e2 e3 : expr),
-        step e1 e1' ->
-        step (E_If e1 e2 e3) (E_If e1' e2 e3)
-    | ST_Let_Left : 
-        ∀ (x : string) (e1 e1' e2 : expr),
-        step e1 e1' ->
-        step (E_Let x e1 e2) (E_Let x e1' e2)
-    | ST_Let_Right : 
-        ∀ (x : string) (v1 e2 e2' : expr),
-        value v1 ->
-        substitution v1 x e2 e2' ->
-        step (E_Let x v1 e2) e2'
-    | ST_Minus_Left :  
-        ∀ (e1 e1' e2 : expr),
-        step e1 e1' ->
-        step (E_Minus e1 e2) (E_Minus e1' e2)
-    | ST_Minus_Right :  
-        ∀ (v1 e2 e2' : expr),
-        value v1 ->
-        step e2 e2' ->
-        step (E_Minus v1 e2) (E_Minus v1 e2')
-    | ST_Minus_Num : 
-        ∀ (z1 z2 : Z),
-        step 
-            (E_Minus (E_Num z1) (E_Num z2))
-            (E_Num (z1 - z2))
-    | ST_Pair_Left :  
-        ∀ (e1 e1' e2 : expr),
-        step e1 e1' ->
-        step (E_Pair e1 e2) (E_Pair e1' e2)
-    | ST_Pair_Right :  
-        ∀ (v1 e2 e2' : expr),
-        value v1 ->
-        step e2 e2' ->
-        step (E_Pair v1 e2) (E_Pair v1 e2')
-    | ST_First :  
-        ∀ (e e' : expr),
-        step e e' ->
-        step (E_First e) (E_First e')
-    | ST_Second :  
-        ∀ (e e' : expr),
-        step e e' ->
-        step (E_Second e) (E_Second e')
-    | ST_First_Pair :  
-        ∀ (v₁ v₂ : expr),
-        value v₁ -> 
-        value v₂ ->
-        step (E_First (E_Pair v₁ v₂)) v₁
-    | ST_Second_Pair :  
-        ∀ (v₁ v₂ : expr),
-        value v₁ -> 
-        value v₂ ->
-        step (E_Second (E_Pair v₁ v₂)) v₂
+  | ST_App_Fun : 
+      ∀ (x : string) (t : type) (e e' v : expr),
+      value v -> 
+      substitution v x e e' ->
+      step (E_App (E_Fun x t e) v) e'
+  | ST_App_Left : 
+      ∀ (e1 e1' e2 : expr),
+      step e1 e1' ->
+      step (E_App e1 e2) (E_App e1' e2)
+  | ST_App_Right : 
+      ∀ (v1 e2 e2' : expr),
+      value v1 ->
+      step e2 e2' ->
+      step (E_App v1 e2) (E_App v1 e2')
+  | ST_If_True : 
+      ∀ (e1 e2 : expr),
+      step (E_If E_True e1 e2) e1
+  | ST_If_False : 
+      ∀ (e1 e2 : expr),
+      step (E_If E_False e1 e2) e2
+  | ST_If : 
+      ∀ (e1 e1' e2 e3 : expr),
+      step e1 e1' ->
+      step (E_If e1 e2 e3) (E_If e1' e2 e3)
+  | ST_Let_Left : 
+      ∀ (x : string) (e1 e1' e2 : expr),
+      step e1 e1' ->
+      step (E_Let x e1 e2) (E_Let x e1' e2)
+  | ST_Let_Right : 
+      ∀ (x : string) (v1 e2 e2' : expr),
+      value v1 ->
+      substitution v1 x e2 e2' ->
+      step (E_Let x v1 e2) e2'
+  | ST_Minus_Left :  
+      ∀ (e1 e1' e2 : expr),
+      step e1 e1' ->
+      step (E_Minus e1 e2) (E_Minus e1' e2)
+  | ST_Minus_Right :  
+      ∀ (v1 e2 e2' : expr),
+      value v1 ->
+      step e2 e2' ->
+      step (E_Minus v1 e2) (E_Minus v1 e2')
+  | ST_Minus_Num : 
+      ∀ (z1 z2 : Z),
+      step 
+          (E_Minus (E_Num z1) (E_Num z2))
+          (E_Num (z1 - z2))
+  | ST_Pair_Left :  
+      ∀ (e1 e1' e2 : expr),
+      step e1 e1' ->
+      step (E_Pair e1 e2) (E_Pair e1' e2)
+  | ST_Pair_Right :  
+      ∀ (v1 e2 e2' : expr),
+      value v1 ->
+      step e2 e2' ->
+      step (E_Pair v1 e2) (E_Pair v1 e2')
+  | ST_First :  
+      ∀ (e e' : expr),
+      step e e' ->
+      step (E_First e) (E_First e')
+  | ST_Second :  
+      ∀ (e e' : expr),
+      step e e' ->
+      step (E_Second e) (E_Second e')
+  | ST_First_Pair :  
+      ∀ (v₁ v₂ : expr),
+      value v₁ -> 
+      value v₂ ->
+      step (E_First (E_Pair v₁ v₂)) v₁
+  | ST_Second_Pair :  
+      ∀ (v₁ v₂ : expr),
+      value v₁ -> 
+      value v₂ ->
+      step (E_Second (E_Pair v₁ v₂)) v₂
+  
+  | ST_Record_Tail : 
+    ∀ x e tail tail', 
+    step tail tail' -> 
+    step (E_Record_Cons x e tail) (E_Record_Cons x e tail')
+  
+  | ST_Record : 
+    ∀ x e e' tail,
+    value tail -> 
+    step e e' -> 
+    step (E_Record_Cons x e tail) (E_Record_Cons x e' tail)
+  
+  | ST_Access : 
+    ∀ x e e',
+    step e e' ->
+    step (E_Record_Access e x) (E_Record_Access e' x)
+
+  | ST_Access_Value : 
+    ∀ x e v,
+    value e -> 
+    lookup_val_record x e = Some v ->
+    step (E_Record_Access e x) v
 .
 
 Hint Constructors step : local_hints.
 
+
+
 Local Lemma not_value: 
-    ∀ e e',
-    value e -> 
-    ~ step e e'.
+  ∀ e e',
+  value e -> 
+  ~ step e e'.
 Proof.
-    induction e; intros e' H_val H_contra;
-    try (inversion H_val; inversion H_contra; fail).
-    inversion H_val; subst.
-    inversion H_contra; subst.
-    - apply IHe1 with e1'; auto.
-    - apply IHe2 with e2'; auto.
+  induction e; intros e' H_val H_contra;
+  try (inversion H_val; inversion H_contra; fail).
+  inversion H_val; subst.
+  inversion H_contra; subst.
+  - apply IHe1 with e1'; auto.
+  - apply IHe2 with e2'; auto.
+  - inversion H_val; subst; inversion H_contra; subst.
+    + eapply IHe2; eauto.
+    + eapply IHe1; eauto.
 Qed.
 
 
 Local Lemma subst_typing : ∀ Γ s x e e' t_e t_s, 
-    has_type (x |-> t_s; Γ) e t_e ->
-    has_type empty s t_s ->
-    substitution s x e e' -> 
-    has_type Γ e' t_e.
+  has_type (x |-> t_s; Γ) e t_e ->
+  has_type empty s t_s ->
+  substitution s x e e' -> 
+  has_type Γ e' t_e.
 Proof.
-    intros * H_type_e H_type_s H_subst.
-    generalize dependent t_e.
-    generalize dependent t_s.
-    generalize dependent Γ.
-    induction H_subst; intros;
-    try (inversion H_type_e; subst; eauto with local_hints; fail).
-    - inversion H_type_e; subst. 
-      rewrite Maps.update_eq in H1. inversion H1; subst. apply Types.weakening_empty.
-      assumption.
-    - inversion H_type_e; subst. 
-      apply T_Var. rewrite Maps.update_neq in H2; auto.
-    - inversion H_type_e; subst.
-      apply T_Fun.   
-      rewrite Maps.update_shadow in H4. assumption.    
-    - inversion H_type_e; subst.
-      apply T_Fun.
-      rewrite Maps.update_permute in H6; auto.
-      eapply IHH_subst; eauto.
+  intros * H_type_e H_type_s H_subst.
+  generalize dependent t_e.
+  generalize dependent t_s.
+  generalize dependent Γ.
+  induction H_subst; intros;
+  try (inversion H_type_e; subst; eauto with local_hints; fail).
+  - inversion H_type_e; subst. 
+    rewrite Maps.update_eq in H1. inversion H1; subst. apply Types.weakening_empty.
+    assumption.
+  - inversion H_type_e; subst. 
+    apply T_Var. rewrite Maps.update_neq in H2; auto.
+  - inversion H_type_e; subst.
+    apply T_Fun.   
+    rewrite Maps.update_shadow in H4. assumption.    
+  - inversion H_type_e; subst.
+    apply T_Fun.
+    rewrite Maps.update_permute in H6; auto.
+    eapply IHH_subst; eauto.
 
-    - inversion H_type_e; subst. eapply T_Let; eauto.
-      rewrite Maps.update_shadow in H5. auto.
-    - inversion H_type_e; subst. eapply T_Let; eauto.
-      rewrite Maps.update_permute in H7; auto.
-      eapply IHH_subst2; eauto.        
+  - inversion H_type_e; subst. eapply T_Let; eauto.
+    rewrite Maps.update_shadow in H5. auto.
+  - inversion H_type_e; subst. eapply T_Let; eauto.
+    rewrite Maps.update_permute in H7; auto.
+    eapply IHH_subst2; eauto.        
 Qed.
 
 Hint Resolve subst_typing : local_hints.
