src/Canonical_form.v
@@ -4,8 +4,9 @@ Require Import Syntax.
 Require Import Types.
 Require Maps.
 
-Local Lemma t_num : ∀ e,
-    has_type empty e Type_Num -> 
+Local Lemma t_num : 
+    ∀ Γ e,
+    has_type Γ e Type_Num -> 
     value e ->
     ∃ z, e = E_Num z.
 Proof.
@@ -16,8 +17,9 @@ Qed.
 
 Hint Resolve t_num : local_hints.
 
-Local Lemma t_bool : ∀ e,
-    has_type empty e Type_Bool -> 
+Local Lemma t_bool : 
+    ∀ Γ e,
+    has_type Γ e Type_Bool -> 
     value e ->
     e = E_True \/ e = E_False.
 Proof.
@@ -28,8 +30,9 @@ Qed.
 
 Hint Resolve t_bool : local_hints.
 
-Local Lemma t_fun : ∀ e t1 t2,
-    has_type empty e (Type_Fun t1 t2) -> 
+Local Lemma t_fun : 
+    ∀ Γ e t1 t2,
+    has_type Γ e (Type_Fun t1 t2) -> 
     value e ->
     ∃ x e', e = E_Fun x t1 e'. 
 Proof.
@@ -42,8 +45,8 @@ Hint Resolve t_fun : local_hints.
 
 
 Local Lemma t_pair :
-    ∀ e t₁ t₂,
-    has_type empty e (Type_Prod t₁ t₂) -> 
+    ∀ Γ e t₁ t₂,
+    has_type Γ e (Type_Prod t₁ t₂) -> 
     value e ->
     ∃ e₁ e₂, e = E_Pair e₁ e₂.
 Proof.
@@ -52,3 +55,94 @@ Proof.
     eauto.
 Qed. 
 Hint Resolve t_pair : local_hints.
+
+
+Local Lemma t_record_nil :
+    ∀ Γ e,
+    has_type Γ e Type_Record_Nil -> 
+    value e ->
+    e = E_Record_Nil.
+Proof.
+    intros * H_type H_val.
+    inversion H_val; subst; try (inversion H_type; fail).
+    reflexivity.
+Qed. 
+
+Hint Resolve t_record_nil : local_hints.
+
+
+Local Lemma t_record_cons :
+    ∀ Γ e x t_x t_tail,
+    has_type Γ e (Type_Record_Cons x t_x t_tail) -> 
+    value e ->
+    ∃ e' e_tail, e = E_Record_Cons x e' e_tail.
+Proof.
+    intros * H_type H_val.
+    inversion H_type; subst; try (inversion H_val; fail).
+    eauto.
+Qed. 
+
+Hint Resolve t_record_cons : local_hints.
+
+
+Local Lemma record_type_exists :
+  ∀ Γ e t_rec t x, 
+  value e ->
+  has_type Γ e t_rec ->
+  lookup_type_record x t_rec = Some t -> 
+  ∃ e', lookup_val_record x e = Some e'.
+Proof.
+  intros Γ e t_rec.
+  generalize dependent Γ.
+  generalize dependent e.
+  induction t_rec; intros;
+  try (inversion H1; fail).
+  simpl in H1.
+  assert (H2 := H0). 
+  apply t_record_cons in H0 as [e' [e_tail H_eq]]; 
+  subst; eauto. 
+  simpl.
+  destruct (String.eqb_spec x0 x); eauto.
+  inversion H; subst.
+  inversion H2.
+  eapply IHt_rec2; eauto.
+Qed.
+
+
+Lemma lookup_type_val :
+  ∀ Γ x e e' t_e t_e',
+  has_type Γ e t_e ->
+  value e ->
+  lookup_type_record x t_e = Some t_e' ->
+  lookup_val_record x e = Some e' -> 
+  has_type Γ e' t_e'.
+Proof.
+  intros Γ x e e' t_e.
+  generalize dependent Γ. 
+  generalize dependent x. 
+  generalize dependent e. 
+  generalize dependent e'.
+  induction t_e; intros; try (inversion H1; fail).
+  simpl in H0.
+  destruct (String.eqb_spec x x0).
+  - symmetry in e0. subst.
+    eapply t_record_cons in H0 as [e'' [e_tail' H_eq']]; 
+    eauto; subst.
+    inversion H; subst. 
+    simpl in H1, H2.
+    rewrite String.eqb_refl in *.
+    inversion H1. inversion H2.
+    subst. auto.    
+  - assert (H_val := H0).
+    eapply t_record_cons in H0 as [e'' [e_tail' H_eq']]; eauto.
+    subst.
+    inversion H_val; subst.
+    inversion H; subst.
+    eapply IHt_e2; 
+    eauto;
+    simpl in *;
+    rewrite <- String.eqb_neq in n;
+    rewrite String.eqb_sym in n;
+    rewrite n in *;
+    eauto.
+Qed.
