src/Closed.v
@@ -20,64 +20,78 @@ e = Minus e1 e2 => x libre dans e1 ou x libre dans e2
  *)
 
 Inductive is_free_in (x : string) : expr -> Prop :=
-| Free_Var : is_free_in x (E_Var x)
-| Free_App_Left : 
-    ∀ e₁ e₂, 
-    is_free_in x e₁ -> 
-    is_free_in x (E_App e₁ e₂) 
-| Free_App_Right : 
-    ∀ e₁ e₂, 
-    is_free_in x e₂ -> 
-    is_free_in x (E_App e₁ e₂) 
-| Free_Fun : 
-    ∀ y t e, 
-    y <> x -> 
+  | Free_Var : is_free_in x (E_Var x)
+  | Free_App_Left : 
+      ∀ e₁ e₂, 
+      is_free_in x e₁ -> 
+      is_free_in x (E_App e₁ e₂) 
+  | Free_App_Right : 
+      ∀ e₁ e₂, 
+      is_free_in x e₂ -> 
+      is_free_in x (E_App e₁ e₂) 
+  | Free_Fun : 
+      ∀ y t e, 
+      y <> x -> 
+      is_free_in x e -> 
+      is_free_in x (E_Fun y t e) 
+  | Free_If_Cond : 
+      ∀ e₁ e₂ e₃, 
+      is_free_in x e₁ -> 
+      is_free_in x (E_If e₁ e₂ e₃) 
+  | Free_If_Left : 
+      ∀ e₁ e₂ e₃, 
+      is_free_in x e₂ -> 
+      is_free_in x (E_If e₁ e₂ e₃) 
+  | Free_If_Right : 
+      ∀ e₁ e₂ e₃, 
+      is_free_in x e₃ -> 
+      is_free_in x (E_If e₁ e₂ e₃) 
+  | Free_Let_Left : 
+      ∀ y e₁ e₂, 
+      is_free_in x e₁ -> 
+      is_free_in x (E_Let y e₁ e₂) 
+  | Free_Let_Right : 
+      ∀ y e₁ e₂, 
+      y <> x -> is_free_in x e₂ -> 
+      is_free_in x (E_Let y e₁ e₂) 
+  | Free_Minus_Left : 
+      ∀ e₁ e₂, 
+      is_free_in x e₁ -> 
+      is_free_in x (E_Minus e₁ e₂) 
+  | Free_Minus_Right : 
+      ∀ e₁ e₂, 
+      is_free_in x e₂ -> 
+      is_free_in x (E_Minus e₁ e₂) 
+  | Free_Pair_Left : 
+      ∀ e₁ e₂, 
+      is_free_in x e₁ -> 
+      is_free_in x (E_Pair e₁ e₂) 
+  | Free_Pair_Right : 
+      ∀ e₁ e₂, 
+      is_free_in x e₂ -> 
+      is_free_in x (E_Pair e₁ e₂) 
+  | Free_First : 
+    ∀ e, 
     is_free_in x e -> 
-    is_free_in x (E_Fun y t e) 
-| Free_If_Cond : 
-    ∀ e₁ e₂ e₃, 
-    is_free_in x e₁ -> 
-    is_free_in x (E_If e₁ e₂ e₃) 
-| Free_If_Left : 
-    ∀ e₁ e₂ e₃, 
-    is_free_in x e₂ -> 
-    is_free_in x (E_If e₁ e₂ e₃) 
-| Free_If_Right : 
-    ∀ e₁ e₂ e₃, 
-    is_free_in x e₃ -> 
-    is_free_in x (E_If e₁ e₂ e₃) 
-| Free_Let_Left : 
-    ∀ y e₁ e₂, 
-    is_free_in x e₁ -> 
-    is_free_in x (E_Let y e₁ e₂) 
-| Free_Let_Right : 
-    ∀ y e₁ e₂, 
-    y <> x -> is_free_in x e₂ -> 
-    is_free_in x (E_Let y e₁ e₂) 
-| Free_Minus_Left : 
-    ∀ e₁ e₂, 
-    is_free_in x e₁ -> 
-    is_free_in x (E_Minus e₁ e₂) 
-| Free_Minus_Right : 
-    ∀ e₁ e₂, 
-    is_free_in x e₂ -> 
-    is_free_in x (E_Minus e₁ e₂) 
-| Free_Pair_Left : 
-    ∀ e₁ e₂, 
-    is_free_in x e₁ -> 
-    is_free_in x (E_Pair e₁ e₂) 
-| Free_Pair_Right : 
-    ∀ e₁ e₂, 
-    is_free_in x e₂ -> 
-    is_free_in x (E_Pair e₁ e₂) 
-| Free_First : 
-  ∀ e, 
-  is_free_in x e -> 
-  is_free_in x (E_First e)
-| Free_Second : 
-  ∀ e, 
-  is_free_in x e -> 
-  is_free_in x (E_Second e)
+    is_free_in x (E_First e)
+  | Free_Second : 
+    ∀ e, 
+    is_free_in x e -> 
+    is_free_in x (E_Second e)
+
+  | Free_Record_Cons_tail :
+    ∀ y e tail, 
+    is_free_in x tail -> 
+    is_free_in x (E_Record_Cons y e tail)
+  | Free_Record_Cons_head :
+    ∀ y e tail, 
+    is_free_in x e -> 
+    is_free_in x (E_Record_Cons y e tail)
+
+  | Free_Record_Access :
+    ∀ y e, 
+      is_free_in x e -> 
+      is_free_in x (E_Record_Access e y) 
 .
 
 Hint Constructors is_free_in : local_hints.
@@ -97,6 +111,8 @@ Proof.
   try (inversion H_type; subst; try eauto; fail);
   try (inversion H_type; subst; erewrite <- Maps.update_neq; eauto; fail).
 Qed. 
+
+Hint Resolve free_has_type : local_hints.
 
 
 Theorem typed_empty :
@@ -118,6 +134,9 @@ Proof.
       rewrite Maps.update_neq in H0; eauto. inversion H0.
 Qed.
 
+Hint Resolve typed_empty : local_hints.
+
+
 Lemma closed_app : 
   ∀ e₁ e₂, 
   closed (E_App e₁ e₂) -> 
@@ -131,6 +150,10 @@ Proof.
     eauto with local_hints.
 Qed.
 
+Hint Resolve closed_app : local_hints.
+
+
+
 Lemma closed_let : 
   ∀ x e₁ e₂, 
   closed (E_Let x e₁ e₂) -> 
@@ -142,6 +165,9 @@ Proof.
   apply H with x'.
   eauto with local_hints.
 Qed.
+
+Hint Resolve closed_let : local_hints.
+
 
 Lemma closed_if : 
   ∀ e₁ e₂ e₃, 
@@ -156,6 +182,9 @@ Proof.
     eauto with local_hints.
 Qed.
 
+Hint Resolve closed_if : local_hints.
+
+
 Lemma closed_minus : 
   ∀ e₁ e₂, 
   closed (E_Minus e₁ e₂) -> 
@@ -168,3 +197,84 @@ Proof.
     apply H with x;
     eauto with local_hints.
 Qed.
+
+Hint Resolve closed_minus : local_hints.
+
+
+
+Lemma closed_pair : 
+  ∀ e₁ e₂, 
+  closed (E_Pair e₁ e₂) -> 
+  closed e₁ /\ closed e₂.
+Proof.
+  intros.
+  unfold closed in *.
+  split; 
+    intros x H_contra;
+    apply H with x;
+    eauto with local_hints.
+Qed.
+
+Hint Resolve closed_pair : local_hints.
+
+Lemma closed_first : 
+  ∀ e, 
+  closed (E_First e) -> 
+  closed e.
+Proof.
+  intros.
+  unfold closed in *.
+  intros x' H_contra;
+  apply H with x';
+  eauto with local_hints.
+Qed.
+Hint Resolve closed_first : local_hints.
+
+
+
+Lemma closed_second : 
+  ∀ e, 
+  closed (E_Second e) -> 
+  closed e.
+Proof.
+  intros.
+  unfold closed in *.
+  intros x' H_contra;
+  apply H with x';
+  eauto with local_hints.
+Qed.
+
+
+Hint Resolve closed_second : local_hints.
+
+
+
+Lemma closed_record : 
+  ∀ x e₁ e₂, 
+  closed (E_Record_Cons x e₁ e₂) -> 
+  closed e₁ /\ closed e₂.
+Proof.
+  intros.
+  unfold closed in *.
+  split; 
+    intros x' H_contra;
+    apply H with x';
+    eauto with local_hints.
+Qed.
+
+Hint Resolve closed_record : local_hints.
+
+
+Lemma closed_access : 
+  ∀ x e, 
+  closed (E_Record_Access e x) -> 
+  closed e.
+Proof.
+  intros.
+  unfold closed in *.
+  intros x' H_contra;
+  apply H with x';
+  eauto with local_hints.
+Qed.
+
+Hint Resolve closed_access : local_hints.
