src/Subst.v
@@ -11,83 +11,98 @@ Require Import Syntax.
 Require Import Types.
 
 Inductive substitution (s : expr) (x : string) : expr -> expr -> Prop :=
-    | S_Var_Eq :
-        substitution s x (E_Var x) s
-    | S_Var_Neq :
-        ∀ (y : string), x <> y -> substitution s x (E_Var y) (E_Var y)
-    | S_App : 
-        ∀ (e1 e1' e2 e2' : expr),
-        substitution s x e1 e1' ->
-        substitution s x e2 e2' ->
-        substitution s x (E_App e1 e2) (E_App e1' e2')
-    | S_Fun_Eq : 
-        ∀ (t : type) (e : expr),
-        substitution s x (E_Fun x t e) (E_Fun x t e)
-    | S_Fun_Neq : 
-        ∀ (y: string) (t : type) (e e_aux e' : expr),
-        x <> y ->
-        closed s ->
-        substitution s x e e' -> 
-        substitution s x (E_Fun y t e) (E_Fun y t e')
-    | S_True : 
-        substitution s x E_True E_True
-    | S_False : 
-        substitution s x E_False E_False
-    | S_If : 
-        ∀ (e1 e1' e2 e2' e3 e3' : expr),
-        substitution s x e1 e1' ->
-        substitution s x e2 e2' ->
-        substitution s x e3 e3' ->
-        substitution s x (E_If e1 e2 e3) (E_If e1' e2' e3')
-    | S_Let_Eq : 
-        ∀ (e1 e1' e2 : expr),
-        substitution s x e1 e1' -> 
-        substitution s x (E_Let x e1 e2) (E_Let x e1' e2)
-    | S_Let_Neq : 
-        ∀ (y : string) (e1 e1' e2 e2': expr),
-        x <> y ->
-        closed s ->
-        substitution s x e1 e1' -> 
-        substitution s x e2 e2' -> 
-        substitution s x (E_Let y e1 e2) (E_Let y e1' e2')
-   
-    | S_Num : 
-        ∀ (z : Z),
-        substitution s x (E_Num z) (E_Num z)
-    | S_Minus :
-        ∀ (e1 e1' e2 e2': expr),
-        substitution s x e1 e1' -> 
-        substitution s x e2 e2' -> 
-        substitution s x (E_Minus e1 e2) (E_Minus e1' e2')
-    | S_Pair : 
-        ∀ (e1 e1' e2 e2': expr),
-        substitution s x e1 e1' -> 
-        substitution s x e2 e2' -> 
-        substitution s x (E_Pair e1 e2) (E_Pair e1' e2')
-    | S_First :
-        ∀ (e e': expr),
-        substitution s x e e' -> 
-        substitution s x (E_First e) (E_First e')
-    | S_Second :
-        ∀ (e e': expr),
-        substitution s x e e' -> 
-        substitution s x (E_Second e) (E_Second e')
+  | S_Var_Eq :
+      substitution s x (E_Var x) s
+  | S_Var_Neq :
+      ∀ (y : string), x <> y -> substitution s x (E_Var y) (E_Var y)
+  | S_App : 
+      ∀ (e1 e1' e2 e2' : expr),
+      substitution s x e1 e1' ->
+      substitution s x e2 e2' ->
+      substitution s x (E_App e1 e2) (E_App e1' e2')
+  | S_Fun_Eq : 
+      ∀ (t : type) (e : expr),
+      substitution s x (E_Fun x t e) (E_Fun x t e)
+  | S_Fun_Neq : 
+      ∀ (y: string) (t : type) (e e_aux e' : expr),
+      x <> y ->
+      closed s ->
+      substitution s x e e' -> 
+      substitution s x (E_Fun y t e) (E_Fun y t e')
+  | S_True : 
+      substitution s x E_True E_True
+  | S_False : 
+      substitution s x E_False E_False
+  | S_If : 
+      ∀ (e1 e1' e2 e2' e3 e3' : expr),
+      substitution s x e1 e1' ->
+      substitution s x e2 e2' ->
+      substitution s x e3 e3' ->
+      substitution s x (E_If e1 e2 e3) (E_If e1' e2' e3')
+  | S_Let_Eq : 
+      ∀ (e1 e1' e2 : expr),
+      substitution s x e1 e1' -> 
+      substitution s x (E_Let x e1 e2) (E_Let x e1' e2)
+  | S_Let_Neq : 
+      ∀ (y : string) (e1 e1' e2 e2': expr),
+      x <> y ->
+      closed s ->
+      substitution s x e1 e1' -> 
+      substitution s x e2 e2' -> 
+      substitution s x (E_Let y e1 e2) (E_Let y e1' e2')
+  
+  | S_Num : 
+      ∀ (z : Z),
+      substitution s x (E_Num z) (E_Num z)
+  | S_Minus :
+      ∀ (e1 e1' e2 e2': expr),
+      substitution s x e1 e1' -> 
+      substitution s x e2 e2' -> 
+      substitution s x (E_Minus e1 e2) (E_Minus e1' e2')
+  | S_Pair : 
+      ∀ (e1 e1' e2 e2': expr),
+      substitution s x e1 e1' -> 
+      substitution s x e2 e2' -> 
+      substitution s x (E_Pair e1 e2) (E_Pair e1' e2')
+  | S_First :
+      ∀ (e e': expr),
+      substitution s x e e' -> 
+      substitution s x (E_First e) (E_First e')
+  | S_Second :
+      ∀ (e e': expr),
+      substitution s x e e' -> 
+      substitution s x (E_Second e) (E_Second e')
+
+  | S_Record_Nil : 
+      substitution s x E_Record_Nil E_Record_Nil
+    
+  | S_Record_Cons :
+    ∀ y e e' tail tail',
+    substitution s x tail tail' ->
+    substitution s x e e' ->
+    substitution s x (E_Record_Cons y e tail) (E_Record_Cons y e' tail')
+  
+  | S_Record_Access :
+    ∀ y e e',
+    substitution s x e e' ->
+    substitution s x (E_Record_Access e y) (E_Record_Access e' y)
+     
 .
 
 Hint Constructors substitution : local_hints.
 
 Local Lemma exists_one : ∀ s x e, closed s -> ∃ e', 
- substitution s x e e'.
+substitution s x e e'.
 Proof with eauto with local_hints.
-    intros.
-    induction e;
-    try (try destruct IHe;
-    try destruct IHe1;
-    try destruct IHe2; 
-    try destruct IHe3; 
-    try destruct (String.eqb_spec x x0); 
-    subst;
-    eauto with local_hints; fail).
+  intros.
+  induction e;
+  try (try destruct IHe;
+  try destruct IHe1;
+  try destruct IHe2; 
+  try destruct IHe3; 
+  try destruct (String.eqb_spec x x0); 
+  subst;
+  eauto with local_hints; fail).
 Qed.
 
 Hint Resolve exists_one : local_hints.
