src/Types.v
@@ -7,93 +7,118 @@ Require Import Syntax.
 Definition context := @Maps.map type.
 Definition empty := @Maps.empty type.
 
+
+
+
 Inductive has_type : context -> expr -> type -> Prop := 
-    | T_Var: 
-        ∀ Γ x t, 
-        Γ ? x = Some t -> 
-        has_type Γ (E_Var x) t
+  (* Base λ-calculus *)
+  | T_Var: 
+      ∀ Γ x t, 
+      Γ ? x = Some t -> 
+      has_type Γ (E_Var x) t
 
-    | T_Fun: 
-        ∀ Γ x t1 e t2,
-        has_type (x |-> t1; Γ) e t2 ->
-        has_type Γ (E_Fun x t1 e) (Type_Fun t1 t2)
+  | T_Fun: 
+      ∀ Γ x t1 e t2,
+      has_type (x |-> t1; Γ) e t2 ->
+      has_type Γ (E_Fun x t1 e) (Type_Fun t1 t2)
 
-    | T_App: 
-        ∀ Γ e1 e2 t1 t2, 
-        has_type Γ e2 t1 -> 
-        has_type Γ e1 (Type_Fun t1 t2) ->
-        has_type Γ (E_App e1 e2) t2
+  | T_App: 
+      ∀ Γ e1 e2 t1 t2, 
+      has_type Γ e2 t1 -> 
+      has_type Γ e1 (Type_Fun t1 t2) ->
+      has_type Γ (E_App e1 e2) t2
 
-    | T_True: 
-        ∀ Γ, 
-        has_type Γ E_True Type_Bool
-                
-    | T_False: 
-        ∀ Γ, 
-        has_type Γ E_False Type_Bool
+  (* Booleans and conditions *)
+  | T_True: 
+      ∀ Γ, 
+      has_type Γ E_True Type_Bool
+              
+  | T_False: 
+      ∀ Γ, 
+      has_type Γ E_False Type_Bool
 
-    | T_If: 
-        ∀ Γ e1 e2 e3 t, 
-        has_type Γ e1 Type_Bool -> 
-        has_type Γ e2 t -> 
-        has_type Γ e3 t -> 
-        has_type Γ (E_If e1 e2 e3) t 
+  | T_If: 
+      ∀ Γ e1 e2 e3 t, 
+      has_type Γ e1 Type_Bool -> 
+      has_type Γ e2 t -> 
+      has_type Γ e3 t -> 
+      has_type Γ (E_If e1 e2 e3) t 
 
-    | T_Let : 
-        ∀ Γ x e1 e2 t1 t2, 
-        has_type Γ e1 t1 -> 
-        has_type (x |-> t1; Γ) e2 t2 -> 
-        has_type Γ (E_Let x e1 e2) t2
+  (* Let expressions *)
+  | T_Let : 
+      ∀ Γ x e1 e2 t1 t2, 
+      has_type Γ e1 t1 -> 
+      has_type (x |-> t1; Γ) e2 t2 -> 
+      has_type Γ (E_Let x e1 e2) t2
 
-    | T_Num : 
-        ∀ Γ z, 
-        has_type Γ (E_Num z) Type_Num 
+  (* Arithmetic *)
+  | T_Num : 
+      ∀ Γ z, 
+      has_type Γ (E_Num z) Type_Num 
 
-    | T_Minus : 
-        ∀ Γ e1 e2, 
-        has_type Γ e1 Type_Num ->
-        has_type Γ e2 Type_Num ->
-        has_type Γ (E_Minus e1 e2) Type_Num 
-    | T_Pair :
-        ∀ Γ e₁ e₂ t₁ t₂, 
-        has_type Γ e₁ t₁ ->
-        has_type Γ e₂ t₂ ->
-        has_type Γ (E_Pair e₁ e₂) (Type_Prod t₁ t₂) 
-    | T_First :
-        ∀ Γ e t₁ t₂,
-        has_type Γ e (Type_Prod t₁ t₂) ->
-        has_type Γ (E_First e) t₁
-    | T_Second :
-        ∀ Γ e t₁ t₂,
-        has_type Γ e (Type_Prod t₁ t₂) ->
-        has_type Γ (E_Second e) t₂
-    .
+  | T_Minus : 
+      ∀ Γ e1 e2, 
+      has_type Γ e1 Type_Num ->
+      has_type Γ e2 Type_Num ->
+      has_type Γ (E_Minus e1 e2) Type_Num 
+
+  (* Pairs *)
+  | T_Pair :
+      ∀ Γ e₁ e₂ t₁ t₂, 
+      has_type Γ e₁ t₁ ->
+      has_type Γ e₂ t₂ ->
+      has_type Γ (E_Pair e₁ e₂) (Type_Prod t₁ t₂) 
+  | T_First :
+      ∀ Γ e t₁ t₂,
+      has_type Γ e (Type_Prod t₁ t₂) ->
+      has_type Γ (E_First e) t₁
+  | T_Second :
+      ∀ Γ e t₁ t₂,
+      has_type Γ e (Type_Prod t₁ t₂) ->
+      has_type Γ (E_Second e) t₂
+
+  (* Records *)
+  | T_Record_Nil :
+      ∀ Γ, has_type Γ E_Record_Nil Type_Record_Nil
+  | T_Record_Cons :
+      ∀ Γ x e tail t_e t_tail, 
+      has_type Γ e t_e -> 
+      has_type Γ tail t_tail -> 
+      record_type t_tail -> 
+      has_type Γ (E_Record_Cons x e tail) (Type_Record_Cons x t_e t_tail) 
+  | T_Record_Access :
+      ∀ Γ x e t_e t_acc, 
+      has_type Γ e t_e -> 
+      lookup_type_record x t_e = Some t_acc ->
+      has_type Γ (E_Record_Access e x) t_acc
+  .
 
 Hint Constructors has_type : local_hints.
 
-
+  
+  
 Local Lemma weakening : ∀ Γ Γ' e t, 
-    Maps.includedin Γ Γ' ->
-    has_type Γ e t ->
-    has_type Γ' e t.
+  Maps.includedin Γ Γ' ->
+  has_type Γ e t ->
+  has_type Γ' e t.
 Proof.
-    intros * H_included H_type.
-    generalize dependent Γ'.
-    induction H_type; intros; eauto with local_hints.
-    - apply T_Fun. apply IHH_type.
-      apply Maps.includedin_update. assumption.
-    - eapply T_Let; eauto. 
-      apply IHH_type2.
-      apply Maps.includedin_update.
-      assumption.
+  intros * H_included H_type.
+  generalize dependent Γ'.
+  induction H_type; intros; eauto with local_hints.
+  - apply T_Fun. apply IHH_type.
+    apply Maps.includedin_update. assumption.
+  - eapply T_Let; eauto. 
+    apply IHH_type2.
+    apply Maps.includedin_update.
+    assumption.
 Qed.
 
 Hint Resolve weakening : local_hints.
 
 
 Local Lemma weakening_empty : ∀ Γ e t, 
-    has_type empty e t ->
-    has_type Γ e t.
+  has_type empty e t ->
+  has_type Γ e t.
 Proof.
 intros. apply (weakening empty); auto.
 intros x v contra. discriminate contra.
